Velvet/Core/NonDet.lean
@@ -2,6 +2,6 @@ module
 
 public import Velvet.Core.NonDet.Findable
 public import Velvet.Core.NonDet.Defs
+public import Velvet.Core.NonDet.Macros
 public import Velvet.Core.NonDet.Run
 public import Velvet.Core.NonDet.WP
-public import Velvet.Core.NonDet.Extract
